add alt composition typing inversion statement, notes

theories/properties.v
@@ -994,6 +994,8 @@ Hint Constructors be_typing : core.
 (** A helper tactic for proving [composition_typing_single]. **)
 Ltac auto_prove_bet:=
   repeat lazymatch goal with
+  | H: _ |- {t3s & (be_typing _ [::] (Tf ?t1s _)) ** _} =>
+    try exists t1s; try eauto
   | H: _ |- {ts & {t1s & {t2s & {t3s & (?tn = ts ++ t1s) ** (?tm = ts ++ t2s) **
                                    (be_typing _ [::] (Tf _ _)) ** _}}}} =>
     try exists [::], tn, tm, tn; try eauto
@@ -1016,11 +1018,75 @@ Proof.
   + by destruct es1 => //=.
   + apply concat_cancel_last in H1. destruct H1. subst.
     by exists [::], t1s0, t2s0, t2s.
-  + edestruct IHHType as [ts' [t1s' [t2s' [t3s' H]]]]; eauto.
+  + (* XXX is this the bet_weakening case?
+     * is this the only case where ts != []?
+     * could it still work with ts = []? *)
+    edestruct IHHType as [ts' [t1s' [t2s' [t3s' H]]]]; eauto.
     destruct H as [->[->[??]]]. 
     exists (ts ++ ts'), t1s', t2s', t3s'.
     by repeat split => //=; rewrite -catA.
 Qed.
+
+Lemma composition_typing_single': forall C es1 e t1s t2s,
+    be_typing C (es1 ++ [::e]) (Tf t1s t2s) ->
+    {t3s &
+      (be_typing C es1 (Tf t1s t3s)) **
+      (be_typing C [::e] (Tf t3s t2s))}.
+Proof.
+  move => C es1 e t1s t2s HType.
+  gen_ind_subst HType; extract_listn; auto_prove_bet.
+  + by apply bet_block.
+  + by destruct es1 => //=.
+  + apply concat_cancel_last in H1. destruct H1. subst.
+    by exists t2s.
+  + edestruct IHHType as [t3s' H]; eauto.
+    destruct H.
+    exists (ts ++ t3s').
+    repeat split; apply bet_weakening with (ts := ts) => //.
+Qed.
+
+Let C_emp := Build_t_context [::] [::] [::] [::] [::] [::] [::] None.
+Let i_add := BI_binop T_i32 (Binop_i BOI_add).
+Let t_ii_to_i := Tf [:: T_i32; T_i32] [:: T_i32].
+Let i_add_typing : be_typing C_emp [:: i_add] t_ii_to_i.
+Proof. apply bet_binop. apply Binop_i32_agree. Qed.
+
+Let t_iii_to_i := Tf [:: T_i32; T_i32; T_i32] [:: T_i32].
+Let seq_2_i_add_typing : be_typing C_emp ([:: i_add] ++ [:: i_add]) t_iii_to_i.
+Proof.
+  apply bet_composition with (t2s := [:: T_i32; T_i32]).
+  - apply bet_weakening with (ts := [:: T_i32]).
+    by apply i_add_typing.
+  - by apply i_add_typing.
+Qed.
+(* proof sketch of the above:
+ *
+ * (1): i_add : ii->i, so by weakening (ts := i) we have i_add : iii->ii
+ *
+ * (2): i_add : ii->i
+ *
+ * to show that [i_add; i_add] : iii->i:
+ *   it's a composition of instrs of types iii->ii and ii->i (by 1,2)
+ *)
+
+Let t_iiiii_to_iii := Tf [:: T_i32; T_i32; T_i32; T_i32; T_i32] [:: T_i32; T_i32; T_i32].
+Let seq_2_i_add_typing' : be_typing C_emp ([:: i_add] ++ [:: i_add]) t_iiiii_to_iii.
+Proof.
+  apply bet_weakening with (ts := [:: T_i32; T_i32]).
+  apply seq_2_i_add_typing.
+Qed.
+
+Definition ts := match composition_typing_single seq_2_i_add_typing with
+                 | existT ts (existT t1s' (existT t2s' (existT t3s _))) =>
+                     (ts, t1s', t2s', t3s)
+                 end.
+(* ([], [i,i,i], [i], [i,i]) *)
+
+Definition ts' := match composition_typing_single seq_2_i_add_typing' with
+                  | existT ts (existT t1s' (existT t2s' (existT t3s _))) =>
+                      (ts, t1s', t2s', t3s)
+                  end.
+(* ([i,i], [i,i,i], [i], [i,i]) *)
 
 Lemma composition_typing: forall C es1 es2 t1s t2s,
     be_typing C (es1 ++ es2) (Tf t1s t2s) ->
